progs/verif_bst.v
@@ -873,7 +873,7 @@ Definition main_spec :=
   POST [ tint ] main_post prog nil gv.
 
 Lemma subsume_insert:
- funspec_sub_weak (snd insert_spec) (snd abs_insert_spec).
+ funspec_sub (snd insert_spec) (snd abs_insert_spec).
 Proof.
 apply NDsubsume_subsume.
 split; reflexivity.
@@ -894,7 +894,7 @@ apply insert_relate; auto.
 Qed.
 
 Lemma subsume_treebox_new:
- funspec_sub_weak (snd treebox_new_spec) (snd abs_treebox_new_spec).
+ funspec_sub (snd treebox_new_spec) (snd abs_treebox_new_spec).
 Proof.
 apply NDsubsume_subsume.
 split; reflexivity.
@@ -918,7 +918,7 @@ simpl. entailer!.
 Qed.
 
 Lemma subsume_treebox_free:
- funspec_sub_weak (snd treebox_free_spec) (snd abs_treebox_free_spec).
+ funspec_sub (snd treebox_free_spec) (snd abs_treebox_free_spec).
 Proof.
 apply NDsubsume_subsume.
 split; reflexivity.
