veric/assert_lemmas.v
@@ -241,7 +241,14 @@ left. destruct H; eauto.
 right. destruct H0; eauto.
 Qed.
 
-Lemma corable_funspec_sub f g: corable (funspec_sub f g).
+Lemma corable_funspec_sub_si f g: corable (funspec_sub_si f g).
+Proof.
+ intros. intro w. destruct f; destruct g. apply prop_ext; split; intro Hx; inv Hx; split; trivial.
++ intros ts. rewrite level_core. specialize (H0 ts); auto.
++ intros ts. specialize (H0 ts). rewrite level_core in H0; auto.
+Qed.
+
+Lemma corable_funspec_sub_early f g: corable (funspec_sub_early f g).
 Proof.
  intros. intro w. destruct f; destruct g. apply prop_ext; split; intro Hx; inv Hx; split; trivial.
 + intros ts. rewrite level_core. specialize (H0 ts); auto.
@@ -286,18 +293,38 @@ Proof.
   apply corable_pureat.
 Qed.
 
-Lemma corable_func_ptr : forall f v, corable (func_ptr f v).
+Lemma corable_func_ptr_si : forall f v, corable (func_ptr_si f v).
 Proof.
   intros.
-  unfold func_ptr.
+  unfold func_ptr_si.
   apply corable_exp; intro.
   apply corable_andp; auto.
   apply corable_exp; intro.
-  apply corable_andp. apply corable_funspec_sub.
+  apply corable_andp. apply corable_funspec_sub_si.
+  apply corable_func_at.
+Qed.
+Lemma corable_func_ptr_early : forall f v, corable (func_ptr_early f v).
+Proof.
+  intros.
+  unfold func_ptr_early.
+  apply corable_exp; intro.
+  apply corable_andp; auto.
+  apply corable_exp; intro.
+  apply corable_andp. apply corable_funspec_sub_early.
+  apply corable_func_at.
+Qed.
+Lemma corable_func_ptr : forall f v, corable (func_ptr f v).
+Proof.
+  intros.
+  unfold func_ptr_early.
+  apply corable_exp; intro.
+  apply corable_andp; auto.
+  apply corable_exp; intro.
+  apply corable_andp. apply corable_prop.
   apply corable_func_at.
 Qed.
 
-Hint Resolve corable_func_ptr.
+Hint Resolve corable_func_ptr corable_func_ptr_si corable_func_ptr_early.
 
 Lemma corable_funspecs_assert:
   forall FS rho, corable (funspecs_assert FS rho).
